@prefix : <http://bimerr.iot.linkeddata.es/def/sensor-data#> .
@prefix owl: <http://www.w3.org/2002/07/owl#> .
@prefix rdf: <http://www.w3.org/1999/02/22-rdf-syntax-ns#> .
@prefix xml: <http://www.w3.org/XML/1998/namespace> .
@prefix xsd: <http://www.w3.org/2001/XMLSchema#> .
@prefix rdfs: <http://www.w3.org/2000/01/rdf-schema#> .
@base <http://bimerr.iot.linkeddata.es/def/sensor-data#> .

<http://bimerr.iot.linkeddata.es/def/sensor-data#> rdf:type owl:Ontology ;
                                                    <http://purl.org/dc/elements/1.1/created> "2020-02-01"@en ;
                                                    <http://purl.org/dc/elements/1.1/creator> "María Poveda-Villalón" ,
                                                                                              "Serge Chávez-Feria." ;
                                                    <http://purl.org/dc/elements/1.1/description> "The Sensor Data ontology has been developed to represent measurements generated by sensors located inside building spaces. It also includes specific concepts and properties to model sensors and actuators records that follow the SenML standard. This model allows the representation of resolved and unresolved records if required. (Check SenML standard for more details: https://tools.ietf.org/html/rfc8428#)"@en ;
                                                    <http://purl.org/dc/elements/1.1/publisher> "http://www.oeg-upm.net/" ;
                                                    <http://purl.org/dc/elements/1.1/title> "Sensor Data ontology"@en ;
                                                    <http://purl.org/dc/terms/license> "http://purl.org/NET/rdflicense/cc-by4.0" ;
                                                    <http://purl.org/vocab/vann/preferredNamespacePrefix> "sd"@en ;
                                                    owl:versionInfo "0.0.3" .

#################################################################
#    Annotation properties
#################################################################

###  http://purl.org/dc/elements/1.1/created
<http://purl.org/dc/elements/1.1/created> rdf:type owl:AnnotationProperty .


###  http://purl.org/dc/elements/1.1/creator
<http://purl.org/dc/elements/1.1/creator> rdf:type owl:AnnotationProperty .


###  http://purl.org/dc/elements/1.1/description
<http://purl.org/dc/elements/1.1/description> rdf:type owl:AnnotationProperty .


###  http://purl.org/dc/elements/1.1/publisher
<http://purl.org/dc/elements/1.1/publisher> rdf:type owl:AnnotationProperty .


###  http://purl.org/dc/elements/1.1/title
<http://purl.org/dc/elements/1.1/title> rdf:type owl:AnnotationProperty .


###  http://purl.org/dc/terms/license
<http://purl.org/dc/terms/license> rdf:type owl:AnnotationProperty .


###  http://purl.org/vocab/vann/preferredNamespacePrefix
<http://purl.org/vocab/vann/preferredNamespacePrefix> rdf:type owl:AnnotationProperty .


###  http://purl.org/vocab/vann/preferredNamespaceUri
<http://purl.org/vocab/vann/preferredNamespaceUri> rdf:type owl:AnnotationProperty .


#################################################################
#    Object Properties
#################################################################

###  https://w3id.org/saref#isControlledByDevice
<https://w3id.org/saref#isControlledByDevice> rdf:type owl:ObjectProperty ;
                                              rdfs:comment "A relationship specifying the devices that can control a certain property."@en ;
                                              rdfs:label "is controlled by device"@en .


###  https://w3id.org/saref#isMeasuredByDevice
<https://w3id.org/saref#isMeasuredByDevice> rdf:type owl:ObjectProperty ;
                                            rdfs:comment "A relationship specifying the devices that can measure a certain property."@en ;
                                            rdfs:label "is measured by device"@en .


###  https://w3id.org/saref#isMeasuredIn
<https://w3id.org/saref#isMeasuredIn> rdf:type owl:ObjectProperty ;
                                      rdfs:comment "A relationship identifying the unit of measure used for a certain entity."@en ;
                                      rdfs:label "is measured in"@en .


###  https://w3id.org/saref#isMeasurementOf
<https://w3id.org/saref#isMeasurementOf> rdf:type owl:ObjectProperty ;
                                         rdfs:comment "A relationship between a measurement and the feature of interest whose quality was measured."@en ;
                                         rdfs:label "is measurement of"@en .


###  https://w3id.org/saref#makesMeasurement
<https://w3id.org/saref#makesMeasurement> rdf:type owl:ObjectProperty ;
                                          rdfs:comment "A relation between a device and the measurements it makes. Such measurement will link together the value of the measurement, its unit of measure and the property to which it relates."@en ;
                                          rdfs:label "makes measurement"@en .


###  https://w3id.org/saref#relatesToProperty
<https://w3id.org/saref#relatesToProperty> rdf:type owl:ObjectProperty ;
                                           rdfs:comment "A relationship between a measurement and the property it relates to."@en ;
                                           rdfs:label "relates to property"@en .


#################################################################
#    Data properties
#################################################################

###  http://bimerr.iot.linkeddata.es/def/sensor-data#baseName
:baseName rdf:type owl:DatatypeProperty ;
          rdfs:domain :Device ;
          rdfs:range xsd:string ;
          rdfs:comment "This is a string that is prepended to the names found in the records."@en ;
          rdfs:label "base name"@en .


###  http://bimerr.iot.linkeddata.es/def/sensor-data#baseSum
:baseSum rdf:type owl:DatatypeProperty ;
         rdfs:domain :Measurement ;
         rdfs:range xsd:double ;
         rdfs:comment "A base sum is added to the sum found in a record."@en ;
         rdfs:label "base sum"@en .


###  http://bimerr.iot.linkeddata.es/def/sensor-data#baseTime
:baseTime rdf:type owl:DatatypeProperty ;
          rdfs:domain :Measurement ;
          rdfs:range xsd:double ;
          rdfs:comment "A base time that is added to the time found in a record."@en ;
          rdfs:label "base time"@en .


###  http://bimerr.iot.linkeddata.es/def/sensor-data#baseValue
:baseValue rdf:type owl:DatatypeProperty ;
           rdfs:domain :Measurement ;
           rdfs:range xsd:double ;
           rdfs:comment "A base value is added to the value found in a record."@en ;
           rdfs:label "base value"@en .


###  http://bimerr.iot.linkeddata.es/def/sensor-data#baseVersion
:baseVersion rdf:type owl:DatatypeProperty ;
             rdfs:domain :Device ;
             rdfs:range xsd:integer ;
             rdfs:comment "Version number of the media type format."@en ;
             rdfs:label "has version"@en .


###  http://bimerr.iot.linkeddata.es/def/sensor-data#name
:name rdf:type owl:DatatypeProperty ;
      rdfs:domain :Device ;
      rdfs:range xsd:string ;
      rdfs:comment "Name of the sensor or parameter.  When appended to the Base Name field, this must result in a globally unique identifier for the resource."@en ;
      rdfs:label "name"@en .


###  http://bimerr.iot.linkeddata.es/def/sensor-data#sum
:sum rdf:type owl:DatatypeProperty ;
     rdfs:domain :Measurement ;
     rdfs:range xsd:double ;
     rdfs:comment "Integrated sum of the values over time.  Optional.  This field is in the unit specified in the Unit value multiplied by seconds."@en ;
     rdfs:label "sum"@en .


###  http://bimerr.iot.linkeddata.es/def/sensor-data#time
:time rdf:type owl:DatatypeProperty ;
      rdfs:domain :Measurement ;
      rdfs:range xsd:double ;
      rdfs:comment "Time when the value was recorded."@en ;
      rdfs:label "time"@en .


###  http://bimerr.iot.linkeddata.es/def/sensor-data#updateTime
:updateTime rdf:type owl:DatatypeProperty ;
            rdfs:domain :Sensor ;
            rdfs:range xsd:double ;
            rdfs:comment "Period of time in seconds that represents the maximum time before this sensor will provide an updated reading for a measurement. This can be used to detect the failure of sensors or the communications path from the sensor."@en ;
            rdfs:label "update time"@en .


###  https://w3id.org/saref#hasValue
<https://w3id.org/saref#hasValue> rdf:type owl:DatatypeProperty ;
                                  rdfs:comment "A relationship defining the value of a certain property, e.g., energy or power. Note that, even if numeric values are expected to enable reasoning, measurement values could use other datatypes."@en ;
                                  rdfs:label "has value"@en .


#################################################################
#    Classes
#################################################################

###  http://bimerr.iot.linkeddata.es/def/building#Element
<http://bimerr.iot.linkeddata.es/def/building#Element> rdf:type owl:Class ;
                                                       rdfs:comment "Building component or construction element which can be described by a set of properties."@en ;
                                                       rdfs:label "Element"@en .


###  http://bimerr.iot.linkeddata.es/def/sensor-data#Actuator
:Actuator rdf:type owl:Class ;
          rdfs:subClassOf :Device ;
          rdfs:comment "A device that is able to receive command signals in the SenML standard, and act over building components in order to change their state."@en ;
          rdfs:label "Actuator"@en .


###  http://bimerr.iot.linkeddata.es/def/sensor-data#Device
:Device rdf:type owl:Class ;
        rdfs:subClassOf <http://bimerr.iot.linkeddata.es/def/building#Element> ,
                        <https://w3id.org/saref#Device> ,
                        [ rdf:type owl:Restriction ;
                          owl:onProperty :baseName ;
                          owl:maxCardinality "1"^^xsd:nonNegativeInteger
                        ] ,
                        [ rdf:type owl:Restriction ;
                          owl:onProperty :baseVersion ;
                          owl:maxCardinality "1"^^xsd:nonNegativeInteger
                        ] ,
                        [ rdf:type owl:Restriction ;
                          owl:onProperty :name ;
                          owl:maxCardinality "1"^^xsd:nonNegativeInteger
                        ] ;
        rdfs:comment "A device that produces or receives records following the SenML standard. A record could mean either a measurement or a control signal."@en ;
        rdfs:label "SenML device"@en .


###  http://bimerr.iot.linkeddata.es/def/sensor-data#Measurement
:Measurement rdf:type owl:Class ;
             rdfs:subClassOf <https://w3id.org/saref#Measurement> ,
                             [ rdf:type owl:Restriction ;
                               owl:onProperty :time ;
                               owl:cardinality "1"^^xsd:nonNegativeInteger
                             ] ,
                             [ rdf:type owl:Restriction ;
                               owl:onProperty :baseSum ;
                               owl:maxCardinality "1"^^xsd:nonNegativeInteger
                             ] ,
                             [ rdf:type owl:Restriction ;
                               owl:onProperty :baseTime ;
                               owl:maxCardinality "1"^^xsd:nonNegativeInteger
                             ] ,
                             [ rdf:type owl:Restriction ;
                               owl:onProperty :baseValue ;
                               owl:maxCardinality "1"^^xsd:nonNegativeInteger
                             ] ,
                             [ rdf:type owl:Restriction ;
                               owl:onProperty :sum ;
                               owl:maxCardinality "1"^^xsd:nonNegativeInteger
                             ] ;
             rdfs:comment "A meaurement or a command signal that follows the SenML specification (https://tools.ietf.org/html/rfc8428)"@en ;
             rdfs:label "SenML record"@en .


###  http://bimerr.iot.linkeddata.es/def/sensor-data#Sensor
:Sensor rdf:type owl:Class ;
        rdfs:subClassOf :Device ,
                        [ rdf:type owl:Restriction ;
                          owl:onProperty :updateTime ;
                          owl:maxCardinality "1"^^xsd:nonNegativeInteger
                        ] ;
        rdfs:comment "A device that is able to produce measurement signals following the SenML standard. A sensor detects and responds to events or changes in the physical environment."@en ;
        rdfs:label "Sensor"@en .


###  https://w3id.org/saref#Device
<https://w3id.org/saref#Device> rdf:type owl:Class ;
                                rdfs:subClassOf [ rdf:type owl:Restriction ;
                                                  owl:onProperty <https://w3id.org/saref#makesMeasurement> ;
                                                  owl:allValuesFrom <https://w3id.org/saref#Measurement>
                                                ] ;
                                rdfs:comment "A tangible object designed to accomplish a particular task. In order to accomplish this task, the device performs one or more functions. For example, a washing machine is designed to wash (task) and to accomplish this task it performs a start and stop function."@en ;
                                rdfs:label "Device"@en .


###  https://w3id.org/saref#FeatureOfInterest
<https://w3id.org/saref#FeatureOfInterest> rdf:type owl:Class ;
                                           rdfs:comment "A feature of interest represents any real world entity from which a property is measured."@en ;
                                           rdfs:label "Feature of interest"@en .


###  https://w3id.org/saref#Measurement
<https://w3id.org/saref#Measurement> rdf:type owl:Class ;
                                     rdfs:subClassOf [ rdf:type owl:Restriction ;
                                                       owl:onProperty <https://w3id.org/saref#isMeasuredIn> ;
                                                       owl:allValuesFrom <https://w3id.org/saref#UnitOfMeasure>
                                                     ] ,
                                                     [ rdf:type owl:Restriction ;
                                                       owl:onProperty <https://w3id.org/saref#isMeasurementOf> ;
                                                       owl:allValuesFrom <https://w3id.org/saref#FeatureOfInterest>
                                                     ] ,
                                                     [ rdf:type owl:Restriction ;
                                                       owl:onProperty <https://w3id.org/saref#relatesToProperty> ;
                                                       owl:allValuesFrom <https://w3id.org/saref#Property>
                                                     ] ,
                                                     [ rdf:type owl:Restriction ;
                                                       owl:onProperty <https://w3id.org/saref#isMeasuredIn> ;
                                                       owl:qualifiedCardinality "1"^^xsd:nonNegativeInteger ;
                                                       owl:onClass <https://w3id.org/saref#UnitOfMeasure>
                                                     ] ,
                                                     [ rdf:type owl:Restriction ;
                                                       owl:onProperty <https://w3id.org/saref#relatesToProperty> ;
                                                       owl:qualifiedCardinality "1"^^xsd:nonNegativeInteger ;
                                                       owl:onClass <https://w3id.org/saref#Property>
                                                     ] ;
                                     rdfs:comment "Represents the measured value made over a property. It is also linked to the unit of measure in which the value is expressed and the timestamp of the measurement."@en ;
                                     rdfs:label "Measurement"@en .


###  https://w3id.org/saref#Property
<https://w3id.org/saref#Property> rdf:type owl:Class ;
                                  rdfs:subClassOf [ rdf:type owl:Restriction ;
                                                    owl:onProperty <https://w3id.org/saref#isControlledByDevice> ;
                                                    owl:allValuesFrom <https://w3id.org/saref#Device>
                                                  ] ,
                                                  [ rdf:type owl:Restriction ;
                                                    owl:onProperty <https://w3id.org/saref#isMeasuredByDevice> ;
                                                    owl:allValuesFrom <https://w3id.org/saref#Device>
                                                  ] ;
                                  rdfs:comment "A quality of a feature of interest that can be measured; an aspect of a feature of interest that is intrinsic to and cannot exist without the feature"@en ;
                                  rdfs:label "Property"@en .


###  https://w3id.org/saref#UnitOfMeasure
<https://w3id.org/saref#UnitOfMeasure> rdf:type owl:Class ;
                                       rdfs:comment "The unit of measure is a standard for measurement of a quantity, such as a Property. For example,  Power is a property and Watt is a unit of power that represents a definite predetermined power: when we say 10 Watt, we actually mean 10 times the definite predetermined power called \\\"watt\\\". Our definition is based on the definition of unit of measure in the Ontology of units of Measure (OM). We propose here a list of some units of measure that are relevant for the purpose of SAREF, but this list can be extended, also using some other ontologies rather than the Ontology of units of Measure (OM)."@en ;
                                       rdfs:label "Unit of measure"@en .


###  Generated by the OWL API (version 5.1.11) https://github.com/owlcs/owlapi/
